Rewrote the compiler to make it easier to work with. Also wrote the syntax for verifiable RTL. Must develop a compiler along those lines next.

PrettyPrintVerilog.hs
@@ -1,6 +1,6 @@
 {-# OPTIONS_GHC -XStandaloneDeriving #-}
 
-import Target hiding (map, concat)
+import Target hiding (map, concat, State, get, put)
 import Data.List
 import Data.List.Split
 import Control.Monad.State.Lazy
@@ -242,11 +242,9 @@ ppRfInstance (_, rf@(RegFile name reads write idxNum dataType init)) =
   "  " ++ ppName name ++ " " ++
   ppName name ++ "$inst(.CLK(CLK), .RESET(RESET), " ++
   concatMap (\read ->
-                ("." ++ ppName read ++ "$_guard(" ++ ppName read ++ "$_guard), ") ++
                 ("." ++ ppName read ++ "$_enable(" ++ ppName read ++ "$_enable), ") ++
                 (ppDealSize0 (Bit (log2_up idxNum)) "" ("." ++ ppName read ++ "$_argument(" ++ ppName read ++ "$_argument), ")) ++
                 ppDealSize0 dataType "" ("." ++ ppName read ++ "$_return(" ++ ppName read ++ "$_return), ")) reads ++
-  ("." ++ ppName write ++ "$_guard(" ++ ppName write ++ "$_guard), ") ++
   ("." ++ ppName write ++ "$_enable(" ++ ppName write ++ "$_enable), ") ++
   ("." ++ ppName write ++ "$_argument(" ++ ppName write ++ "$_argument)") ++
   ");\n\n"
@@ -254,11 +252,9 @@ ppRfInstance (_, rf@(RegFileFile name reads write idxNum dataType file isAscii))
   "  " ++ ppName name ++ " " ++
   ppName name ++ "$inst(.CLK(CLK), .RESET(RESET), " ++
   concatMap (\read ->
-                ("." ++ ppName read ++ "$_guard(" ++ ppName read ++ "$_guard), ") ++
                 ("." ++ ppName read ++ "$_enable(" ++ ppName read ++ "$_enable), ") ++
                 (ppDealSize0 (Bit (log2_up idxNum)) "" ("." ++ ppName read ++ "$_argument(" ++ ppName read ++ "$_argument), ")) ++
                 ppDealSize0 dataType "" ("." ++ ppName read ++ "$_return(" ++ ppName read ++ "$_return), ")) reads ++
-  ("." ++ ppName write ++ "$_guard(" ++ ppName write ++ "$_guard), ") ++
   ("." ++ ppName write ++ "$_enable(" ++ ppName write ++ "$_enable), ") ++
   ("." ++ ppName write ++ "$_argument(" ++ ppName write ++ "$_argument)") ++
   ");\n\n"
@@ -266,16 +262,13 @@ ppRfInstance (_, rf@(SyncRegFile isAddr name reads write idxNum dataType init)) 
   "  " ++ ppName name ++ " " ++
   ppName name ++ "$inst(.CLK(CLK), .RESET(RESET), " ++
   concatMap (\((read, readRs), _) ->
-                ("." ++ ppName read ++ "$_guard(" ++ ppName read ++ "$_guard), ") ++
                 ("." ++ ppName read ++ "$_enable(" ++ ppName read ++ "$_enable), ") ++
                 (ppDealSize0 (Bit (log2_up idxNum)) "" ("." ++ ppName read ++ "$_argument(" ++ ppName read ++ "$_argument), ")) ++
                 ppDealSize0 dataType "" ("." ++ ppName read ++ "$_return(" ++ ppName read ++ "$_return), ") ++
-                ("." ++ ppName readRs ++ "$_guard(" ++ ppName readRs ++ "$_guard), ") ++
                 ("." ++ ppName readRs ++ "$_enable(" ++ ppName readRs ++ "$_enable), ") ++
                 (ppDealSize0 (Bit (log2_up idxNum)) "" ("." ++ ppName readRs ++ "$_argument(" ++ ppName readRs ++ "$_argument), ")) ++
                 ppDealSize0 dataType "" ("." ++ ppName readRs ++ "$_return(" ++ ppName readRs ++ "$_return), ")
             ) reads ++
-  ("." ++ ppName write ++ "$_guard(" ++ ppName write ++ "$_guard), ") ++
   ("." ++ ppName write ++ "$_enable(" ++ ppName write ++ "$_enable), ") ++
   ("." ++ ppName write ++ "$_argument(" ++ ppName write ++ "$_argument)") ++
   ");\n\n"
@@ -283,16 +276,13 @@ ppRfInstance (_, rf@(SyncRegFileFile isAddr name reads write idxNum dataType fil
   "  " ++ ppName name ++ " " ++
   ppName name ++ "$inst(.CLK(CLK), .RESET(RESET), " ++
   concatMap (\((read, readRs), _) ->
-                ("." ++ ppName read ++ "$_guard(" ++ ppName read ++ "$_guard), ") ++
                 ("." ++ ppName read ++ "$_enable(" ++ ppName read ++ "$_enable), ") ++
                 (ppDealSize0 (Bit (log2_up idxNum)) "" ("." ++ ppName read ++ "$_argument(" ++ ppName read ++ "$_argument), ")) ++
                 ppDealSize0 dataType "" ("." ++ ppName read ++ "$_return(" ++ ppName read ++ "$_return), ") ++
-                ("." ++ ppName readRs ++ "$_guard(" ++ ppName readRs ++ "$_guard), ") ++
                 ("." ++ ppName readRs ++ "$_enable(" ++ ppName readRs ++ "$_enable), ") ++
                 (ppDealSize0 (Bit (log2_up idxNum)) "" ("." ++ ppName readRs ++ "$_argument(" ++ ppName readRs ++ "$_argument), ")) ++
                 ppDealSize0 dataType "" ("." ++ ppName readRs ++ "$_return(" ++ ppName readRs ++ "$_return), ")
             ) reads ++
-  ("." ++ ppName write ++ "$_guard(" ++ ppName write ++ "$_guard), ") ++
   ("." ++ ppName write ++ "$_enable(" ++ ppName write ++ "$_enable), ") ++
   ("." ++ ppName write ++ "$_argument(" ++ ppName write ++ "$_argument)") ++
   ");\n\n"
@@ -301,18 +291,15 @@ ppRfModule :: (Bool, RegFileBase) -> String
 ppRfModule (bypass, rf@(RegFile name reads write idxNum dataType init)) =
   "module " ++ ppName name ++ "(\n" ++
   concatMap (\read ->
-               ("  output " ++ ppDeclType (ppName read ++ "$_guard") Bool ++ ",\n") ++
                ("  input " ++ ppDeclType (ppName read ++ "$_enable") Bool ++ ",\n") ++
                (ppDealSize0 (Bit (log2_up idxNum)) "" ("  input " ++ ppDeclType (ppName read ++ "$_argument") (Bit (log2_up idxNum)) ++ ",\n")) ++
                ppDealSize0 dataType "" ("  output " ++ ppDeclType (ppName read ++ "$_return") dataType ++ ",\n")) reads ++
-  ("  output " ++ ppDeclType (ppName write ++ "$_guard") Bool ++ ",\n") ++
   ("  input " ++ ppDeclType (ppName write ++ "$_enable") Bool ++ ",\n") ++
   ppDealSize0 (writeRegFile idxNum dataType) "" (("  input " ++ ppDeclType (ppName write ++ "$_argument") (writeRegFile idxNum dataType) ++ ",\n")) ++
   "  input logic CLK,\n" ++
   "  input logic RESET\n" ++
   ");\n" ++
   ppDealSize0 dataType "" ("  " ++ ppDeclType (ppName name ++ "$_data") dataType ++ "[0:" ++ show (idxNum - 1) ++ "];\n") ++
-  "  assign " ++ ppName write ++ "$_guard = 1'b1;\n" ++
   (case init of
      Just initVal ->
        "  initial begin\n" ++
@@ -322,7 +309,6 @@ ppRfModule (bypass, rf@(RegFile name reads write idxNum dataType init)) =
        "  end\n"
      Nothing -> "") ++
   concatMap (\read ->
-               "  assign " ++ ppName read ++ "$_guard = 1'b1;\n" ++
                ppDealSize0 dataType "" ("  assign " ++ ppName read ++ "$_return = " ++
                                         (if bypass
                                          then ppName write ++ "$_enable && " ++ ppName write ++ "$_argument.addr == " ++
@@ -346,24 +332,20 @@ ppRfModule (bypass, rf@(RegFile name reads write idxNum dataType init)) =
 ppRfModule (bypass, rf@(RegFileFile name reads write idxNum dataType file isAscii)) =
   "module " ++ ppName name ++ "(\n" ++
   concatMap (\read ->
-               ("  output " ++ ppDeclType (ppName read ++ "$_guard") Bool ++ ",\n") ++
                ("  input " ++ ppDeclType (ppName read ++ "$_enable") Bool ++ ",\n") ++
                (ppDealSize0 (Bit (log2_up idxNum)) "" ("  input " ++ ppDeclType (ppName read ++ "$_argument") (Bit (log2_up idxNum)) ++ ",\n")) ++
                ppDealSize0 dataType "" ("  output " ++ ppDeclType (ppName read ++ "$_return") dataType ++ ",\n")) reads ++
-  ("  output " ++ ppDeclType (ppName write ++ "$_guard") Bool ++ ",\n") ++
   ("  input " ++ ppDeclType (ppName write ++ "$_enable") Bool ++ ",\n") ++
   ppDealSize0 (writeRegFile idxNum dataType) "" (("  input " ++ ppDeclType (ppName write ++ "$_argument") (writeRegFile idxNum dataType) ++ ",\n")) ++
   "  input logic CLK,\n" ++
   "  input logic RESET\n" ++
   ");\n" ++
   ppDealSize0 dataType "" ("  " ++ ppDeclType (ppName name ++ "$_data") dataType ++ "[0:" ++ show (idxNum - 1) ++ "];\n") ++
-  "  assign " ++ ppName write ++ "$_guard = 1'b1;\n" ++
   "  initial begin\n" ++
   "    $readmem" ++ (if isAscii then "h" else "b") ++ "(\"" ++ file ++ "\"," ++ ppName name ++ "$_data"++ ");\n" ++
   "    end\n" ++
   "  end\n" ++
   concatMap (\read ->
-               "  assign " ++ ppName read ++ "$_guard = 1'b1;\n" ++
                ppDealSize0 dataType "" ("  assign " ++ ppName read ++ "$_return = " ++
                                         (if bypass
                                          then ppName write ++ "$_enable && " ++ ppName write ++ "$_argument.addr == " ++
@@ -381,17 +363,20 @@ ppRfModule x = undefined
 removeDups :: Eq a => [(a, b)] -> [(a, b)]
 removeDups = nubBy (\(a, _) (b, _) -> a == b)
 
+getAllMethodsRegFileList :: [RegFileBase] -> [(String, (Kind, Kind))]
+getAllMethodsRegFileList ls = map (\(x, (y, z)) -> (x, y)) (concat (map (\x -> getMethods (BaseRegFile x)) ls))
+
+
+
 ppRtlInstance :: RtlModule -> String
 ppRtlInstance m@(Build_RtlModule hiddenWires regFs ins' outs' regInits' regWrites' assigns' sys') =
   "  _design _designInst(.CLK(CLK), .RESET(RESET)" ++
   concatMap (\(nm, ty) -> ppDealSize0 ty "" (", ." ++ ppPrintVar nm ++ '(' : ppPrintVar nm ++ ")")) (removeDups ins' ++ removeDups outs') ++
   concatMap (\(nm, ty) -> ppDealSize0 ty "" (", ." ++ ppPrintVar nm ++ '(' : ppPrintVar nm ++ ")")) rfMeths ++ ");\n"
   where
-    rfMeths = Data.List.map (\x -> ((fst x ++ "#_argument", []), fst (fst (snd x))) ) (getAllMethodsRegFileList (map snd regFs)) ++
-              Data.List.map (\x -> ((fst x ++ "#_return", []), snd (fst (snd x))) ) (getAllMethodsRegFileList (map snd regFs)) ++
-              Data.List.map (\x -> ((fst x ++ "#_enable", []), Bool) ) (getAllMethodsRegFileList (map snd regFs)) ++
-              Data.List.map (\x -> ((fst x ++ "#_guard", []), Bool) ) (getAllMethodsRegFileList (map snd regFs))
-
+    rfMeths = Data.List.map (\x -> ((fst x ++ "#_argument", []), fst (snd x)) ) (getAllMethodsRegFileList (map snd regFs)) ++
+              Data.List.map (\x -> ((fst x ++ "#_return", []), snd (snd x)) ) (getAllMethodsRegFileList (map snd regFs)) ++
+              Data.List.map (\x -> ((fst x ++ "#_enable", []), Bool) ) (getAllMethodsRegFileList (map snd regFs))
 ppBitFormat :: BitFormat -> String
 ppBitFormat Binary = "b"
 ppBitFormat Decimal = "d"
@@ -469,9 +454,8 @@ ppRtlModule m@(Build_RtlModule hiddenWires regFs ins' outs' regInits' regWrites'
     regInits = removeDups regInits'
     regWrites = removeDups regWrites'
     assigns = removeDups assigns'
-    rfMethsIn = Data.List.map (\x -> ((fst x ++ "#_return", []), snd (fst (snd x))) ) (getAllMethodsRegFileList (map snd regFs)) ++
-                Data.List.map (\x -> ((fst x ++ "#_guard", []), Bool) ) (getAllMethodsRegFileList (map snd regFs))
-    rfMethsOut = Data.List.map (\x -> ((fst x ++ "#_argument", []), fst (fst (snd x))) ) (getAllMethodsRegFileList (map snd regFs)) ++
+    rfMethsIn = Data.List.map (\x -> ((fst x ++ "#_return", []), snd (snd x)) ) (getAllMethodsRegFileList (map snd regFs))
+    rfMethsOut = Data.List.map (\x -> ((fst x ++ "#_argument", []), fst (snd x)) ) (getAllMethodsRegFileList (map snd regFs)) ++
                  Data.List.map (\x -> ((fst x ++ "#_enable", []), Bool) ) (getAllMethodsRegFileList (map snd regFs))
     convAssigns =
       mapM (\(nm, (ty, expr)) ->
@@ -542,11 +526,10 @@ ppTopModule m@(Build_RtlModule hiddenWires regFs ins' outs' regInits' regWrites'
     isHidden (x, _) = not (elem x hiddenWires)
     insFiltered = Data.List.filter isHidden ins
     outsFiltered = Data.List.filter isHidden outs
-    rfMeths = Data.List.map (\x -> ((fst x ++ "#_argument", []), fst (fst (snd x))) ) (getAllMethodsRegFileList (map snd regFs)) ++
-              Data.List.map (\x -> ((fst x ++ "#_return", []), snd (fst (snd x))) ) (getAllMethodsRegFileList (map snd regFs)) ++
-              Data.List.map (\x -> ((fst x ++ "#_enable", []), Bool) ) (getAllMethodsRegFileList (map snd regFs)) ++
-              Data.List.map (\x -> ((fst x ++ "#_guard", []), Bool) ) (getAllMethodsRegFileList (map snd regFs))
-
+    rfMeths = Data.List.map (\x -> ((fst x ++ "#_argument", []), fst (snd x)) ) (getAllMethodsRegFileList (map snd regFs)) ++
+              Data.List.map (\x -> ((fst x ++ "#_return", []), snd (snd x)) ) (getAllMethodsRegFileList (map snd regFs)) ++
+              Data.List.map (\x -> ((fst x ++ "#_enable", []), Bool) ) (getAllMethodsRegFileList (map snd regFs))
+              
 printDiff :: [(String, [String])] -> [(String, [String])] -> IO ()
 printDiff (x:xs) (y:ys) =
   do
