CompileOld.v
@@ -1,0 +1,646 @@
+Require Import Syntax Rtl.
+
+Set Implicit Arguments.
+Set Asymmetric Patterns.
+
+Local Open Scope string.
+
+Local Notation nil_nat := (nil: list nat).
+
+Definition getRegActionRead a s := (a ++ "#" ++ s ++ "#_read", nil_nat).
+Definition getRegActionWrite a s := (a ++ "#" ++ s ++ "#_tempwrite", nil_nat).
+Definition getRegActionFinalWrite a s := (a ++ "#" ++ s ++ "#_write", nil_nat).
+Definition getRegActionEn a s := (a ++ "#" ++ s ++ "#_en", nil_nat).
+
+Definition getRegRead s := (s ++ "#_read", nil_nat).
+Definition getRegWrite s := (s ++ "#_write", nil_nat).
+
+Definition getMethActionArg a f := (a ++ "#" ++ f ++ "#_argument", nil_nat).
+Definition getMethActionEn a f := (a ++ "#" ++ f ++ "#_enable", nil_nat).
+
+Definition getMethRet f := (f ++ "#_return", nil_nat).
+Definition getMethArg f := (f ++ "#_argument", nil_nat).
+Definition getMethEn f := (f ++ "#_enable", nil_nat).
+Definition getMethGuard f := (f ++ "#_guard", nil_nat).
+
+Definition getActionGuard r := (r ++ "#_guard", nil_nat).
+Definition getActionEn r := (r ++ "#_enable", nil_nat).
+
+Local Close Scope string.
+
+Local Notation cast k' v := v (only parsing).
+
+
+Section Compile.
+  Variable name: string.
+
+  Fixpoint convertExprToRtl k (e: Expr (fun _ => list nat) (SyntaxKind k)) :=
+    match e in Expr _ (SyntaxKind k) return RtlExpr k with
+      | Var k' x' =>   match k' return
+                             (forall x,
+                                match k' return (Expr (fun _ => list nat) k' -> Set) with
+                                  | SyntaxKind k => fun _ => RtlExpr k
+                                  | NativeKind _ => fun _ => IDProp
+                                end (Var (fun _ => list nat) k' x))
+                       with
+                         | SyntaxKind k => fun x => RtlReadWire k (name, x)
+                         | NativeKind t => fun _ => idProp
+                       end x'
+      | Const k x => RtlConst x
+      | UniBool x x0 => RtlUniBool x (@convertExprToRtl _ x0)
+      | CABool x x0 => RtlCABool x (map (@convertExprToRtl _) x0)
+      | UniBit n1 n2 x x0 => RtlUniBit x (@convertExprToRtl _ x0)
+      | CABit n x x0 => RtlCABit x (map (@convertExprToRtl _) x0)
+      | BinBit n1 n2 n3 x x0 x1 => RtlBinBit x (@convertExprToRtl _ x0) (@convertExprToRtl _ x1)
+      | BinBitBool n1 n2 x x0 x1 => RtlBinBitBool x (@convertExprToRtl _ x0) (@convertExprToRtl _ x1)
+      | Eq k e1 e2 => RtlEq (@convertExprToRtl _ e1) (@convertExprToRtl _ e2)
+      | ReadStruct n fk fs e i => @RtlReadStruct n fk fs (@convertExprToRtl _ e) i
+      | BuildStruct n fk fs fv => @RtlBuildStruct n fk fs (fun i => @convertExprToRtl _ (fv i))
+      | ReadArray n k arr idx => @RtlReadArray n k (@convertExprToRtl _ arr) (@convertExprToRtl _ idx)
+      | ReadArrayConst n k arr idx => @RtlReadArrayConst n k (@convertExprToRtl _ arr) idx
+      | BuildArray n k farr => @RtlBuildArray n k (fun i => @convertExprToRtl _ (farr i))
+      | ITE k' x x0' x1' =>
+        match k' return
+              (forall x0 x1,
+                 match k' return (Expr (fun _ => list nat) k' -> Set) with
+                   | SyntaxKind k => fun _ => RtlExpr k
+                   | NativeKind _ => fun _ => IDProp
+                 end (ITE x x0 x1))
+        with
+          | SyntaxKind k => fun x0 x1 => RtlITE (@convertExprToRtl _ x) (@convertExprToRtl _ x0) (@convertExprToRtl _ x1)
+          | NativeKind t => fun _ _ => idProp
+        end x0' x1'
+    end.
+
+  Local Definition inc ns := match ns with
+                             | nil => nil
+                             | x :: xs => S x :: xs
+                             end.
+
+  Axiom cheat: forall t, t.
+
+  Fixpoint convertActionToRtl_noGuard k (a: ActionT (fun _ => list nat) k) startList retList :=
+    match a in ActionT _ _ with
+      | MCall meth k argExpr cont =>
+        (name, startList, existT _ (snd k) (RtlReadWire (snd k) (getMethRet meth))) ::
+        convertActionToRtl_noGuard (cont startList) (inc startList) retList
+      | Return x => (name, retList, existT _ k (convertExprToRtl x)) :: nil
+      | LetExpr k' expr cont =>
+        match k' return Expr (fun _ => list nat) k' ->
+                        (fullType (fun _ => list nat) k' -> ActionT (fun _ => list nat) k) ->
+                        list (string * list nat * sigT RtlExpr) with
+        | SyntaxKind k => fun expr cont => (name, startList, existT _ k (convertExprToRtl expr))
+                                             ::
+                                             convertActionToRtl_noGuard (cont startList) (inc startList)
+                                             retList
+        | _ => fun _ _ => nil
+        end expr cont
+      | LetAction k' a' cont =>
+        convertActionToRtl_noGuard a' (0 :: startList) startList ++
+        convertActionToRtl_noGuard (cont startList) (inc startList) retList
+      | ReadNondet k' cont =>
+        match k' return (fullType (fun _ => list nat) k' -> ActionT (fun _ => list nat) k) ->
+                        list (string * list nat * sigT RtlExpr) with
+        | SyntaxKind k => fun cont => (name, startList, existT _ k (convertExprToRtl
+                                                                      (Const _ (getDefaultConst _))))
+                                        ::
+                                        convertActionToRtl_noGuard (cont startList) (inc startList) retList
+        | _ => fun _ => nil
+        end cont
+      | ReadReg r k' cont =>
+        match k' return (fullType (fun _ => list nat) k' -> ActionT (fun _ => list nat) k) ->
+                        list (string * list nat * sigT RtlExpr) with
+          | SyntaxKind k => fun cont => (name, startList,
+                                         existT _ k (RtlReadWire k (getRegActionRead name r)))
+                                          ::
+                                          convertActionToRtl_noGuard (cont startList)
+                                          (inc startList) retList
+          | _ => fun _ => nil
+        end cont
+      | WriteReg r k' expr cont =>
+        convertActionToRtl_noGuard cont startList retList
+      | Assertion pred cont => convertActionToRtl_noGuard cont startList retList
+      | Sys ls cont => convertActionToRtl_noGuard cont startList retList
+      | IfElse pred ktf t f cont =>
+        convertActionToRtl_noGuard t (0 :: startList) (startList) ++
+        convertActionToRtl_noGuard f (0 :: inc startList) (inc startList) ++
+          (name, inc (inc startList),
+           existT _ ktf (RtlITE (convertExprToRtl pred) (RtlReadWire ktf (name, startList)) (RtlReadWire ktf (name, inc startList)))) ::
+        convertActionToRtl_noGuard (cont (inc (inc startList))) (inc (inc (inc startList))) retList
+        end.
+
+  Fixpoint convertActionToRtl_guard k (a: ActionT (fun _ => list nat) k) startList:
+    list (RtlExpr Bool) :=
+    match a in ActionT _ _ with
+      | MCall meth k argExpr cont =>
+        RtlReadWire Bool (getActionGuard meth) ::
+                    (convertActionToRtl_guard (cont startList) (inc startList))
+      | LetExpr k' expr cont =>
+        match k' return (fullType (fun _ => list nat) k' -> ActionT (fun _ => list nat) k) ->
+                        list (RtlExpr Bool) with
+        | SyntaxKind k => fun cont =>
+                            convertActionToRtl_guard (cont startList) (inc startList)
+        | _ => fun _ => nil
+        end cont
+      | ReadNondet k' cont =>
+        match k' return (fullType (fun _ => list nat) k' -> ActionT (fun _ => list nat) k) ->
+                        list (RtlExpr Bool) with
+        | SyntaxKind k => fun cont =>
+                            convertActionToRtl_guard (cont startList) (inc startList)
+        | _ => fun _ => nil
+        end cont
+      | ReadReg r k' cont =>
+        match k' return (fullType (fun _ => list nat) k' -> ActionT (fun _ => list nat) k) ->
+                        list (RtlExpr Bool) with
+        | SyntaxKind k => fun cont =>
+                            convertActionToRtl_guard (cont startList) (inc startList)
+        | _ => fun _ => nil
+        end cont
+      | WriteReg r k' expr cont =>
+        convertActionToRtl_guard cont startList
+      | Assertion pred cont => convertExprToRtl pred ::
+                                              (convertActionToRtl_guard cont startList)
+      | Sys ls cont => convertActionToRtl_guard cont startList
+      | Return x => nil
+      | IfElse pred ktf t f cont =>
+        let wc := convertActionToRtl_guard (cont (inc (inc startList))) (inc (inc (inc startList))) in
+        let p := convertExprToRtl pred in
+        match convertActionToRtl_guard t (0 :: startList), convertActionToRtl_guard f (0 :: inc startList) with
+        | nil, nil => wc
+        | e, nil => RtlCABool Or (RtlUniBool Neg p :: e) :: wc
+        | nil, e => RtlCABool Or (p :: e) :: wc
+        | e1, e2 => RtlITE p (RtlCABool And e1) (RtlCABool And e2) :: wc
+        end
+        (* (RtlITE (convertExprToRtl pred) (RtlCABool And *)
+        (*                                            (convertActionToRtl_guard t (0 :: startList))) *)
+        (*         (RtlCABool And (convertActionToRtl_guard f (0 :: inc startList)))) *)
+        (*   :: *)
+        (*   (convertActionToRtl_guard (cont (inc (inc startList))) *)
+        (*                             (inc (inc (inc startList)))) *)
+      | LetAction k' a' cont =>
+        convertActionToRtl_guard a' (0 :: startList) ++
+                                 convertActionToRtl_guard (cont startList) (inc startList)
+    end.
+
+  Definition convertActionToRtl_guardF k (a: ActionT (fun _ => list nat) k) startList :=
+    RtlCABool And (convertActionToRtl_guard a startList).
+
+  Definition invalidRtl k v :=
+    ((STRUCT {
+          "valid" ::= RtlConst false ;
+          "data" ::= v
+     })%rtl_expr : RtlExpr (Maybe k)).
+
+
+  Definition conditionPair k (p: RtlExpr Bool) (e1 e2: (RtlExpr Bool * RtlExpr k)) :=
+    (RtlITE p (fst e1) (fst e2), RtlITE p (snd e1) (snd e2)).
+  Definition invalidPair k (v: RtlExpr k) := (RtlConst false, v).
+             
+  Section MethReg.
+    Open Scope string.
+    Section GetRegisterWrites.
+      Variable reg: RegInitT.
+      
+      Definition regKind := match projT1 (snd reg) with
+                            | SyntaxKind k => k
+                            | _ => Void
+                            end.
+      
+      Fixpoint getRegisterWrites k (a: ActionT (fun _ => list nat) k) (startList: list nat) : sum (RtlExpr Bool * RtlExpr regKind) (RtlExpr regKind) :=
+        match a in ActionT _ _ with
+        | MCall meth k argExpr cont =>
+          @getRegisterWrites _ (cont startList) (inc startList)
+        | Return x => inr (RtlConst (getDefaultConst _))
+        | LetExpr k' expr cont =>
+          match k' return Expr (fun _ => list nat) k' ->
+                          (fullType (fun _ => list nat) k' -> ActionT (fun _ => list nat) k) -> _ with
+          | SyntaxKind k => fun expr cont => @getRegisterWrites _ (cont startList) (inc startList)
+          | _ => fun _ _ => inr (RtlConst (getDefaultConst _))
+          end expr cont
+        | LetAction k' a' cont =>
+          let w1 := @getRegisterWrites _ a' (0 :: startList) in
+          let w2 := @getRegisterWrites _ (cont startList) (inc startList) in
+          match w1, w2 with
+          | inr x, inr y => inr x
+          | inr _, inl w2' => inl w2'
+          | inl w1', inr _ => inl w1'
+          | inl w1', inl w2' => inl (conditionPair (fst w2') w2' w1')%rtl_expr
+          end
+        | ReadNondet k' cont =>
+          match k' return (fullType (fun _ => list nat) k' -> ActionT (fun _ => list nat) k) -> _ with
+          | SyntaxKind k => fun cont => @getRegisterWrites _ (cont startList) (inc startList)
+          | _ => fun _ => inr (RtlConst (getDefaultConst _))
+          end cont
+        | ReadReg r k' cont =>
+          match k' return (fullType (fun _ => list nat) k' -> ActionT (fun _ => list nat) k) -> _ with
+          | SyntaxKind k => fun cont => @getRegisterWrites _ (cont startList) (inc startList)
+          | _ => fun _ => inr (RtlConst (getDefaultConst _))
+          end cont
+        | Assertion pred cont => @getRegisterWrites _ cont startList
+        | Sys ls cont => @getRegisterWrites _ cont startList
+        | IfElse pred ktf t f cont =>
+          let p := convertExprToRtl pred in
+          let wt := @getRegisterWrites _ t (0 :: startList) in
+          let wf := @getRegisterWrites _ f (0 :: inc startList) in
+          let wc := @getRegisterWrites _ (cont (inc (inc startList))) (inc (inc (inc startList))) in
+          match wt, wf, wc with
+          | inr x, inr y, inr z => inr x
+          | inr x, inr y, inl wc' => inl wc'
+          | inr x, inl wf', inr z => inl (conditionPair p (invalidPair (snd wf')) wf')
+          | inl wt', inr y, inr z => inl (conditionPair p wt' (invalidPair (snd wt')))
+          | inl wt', inl wf', inr z => inl (conditionPair p wt' wf')
+          | inl wt', inr y, inl wc' => inl (conditionPair (fst wc') wc' (conditionPair p wt' (invalidPair (snd wt'))))%rtl_expr
+          | inr x, inl wf', inl wc' => inl (conditionPair (fst wc') wc' (conditionPair p (invalidPair (snd wf')) wf'))%rtl_expr
+          | inl wt', inl wf', inl wc' => inl (conditionPair (fst wc') wc'
+                                                            (conditionPair p wt' wf'))%rtl_expr
+          end
+        | WriteReg r k' expr cont =>
+          let wc := @getRegisterWrites _ cont startList in
+          if string_dec r (fst reg)
+          then
+            match k' return Expr (fun _ => list nat) k' -> sum (RtlExpr Bool * RtlExpr regKind) (RtlExpr regKind) with
+            | SyntaxKind k => fun expr =>
+                                match Kind_dec regKind k with
+                                | left pf => match pf in _ = Y return Expr _ (SyntaxKind Y) -> sum (RtlExpr Bool * RtlExpr regKind) (RtlExpr regKind) with
+                                             | eq_refl => fun expr =>
+                                                            match wc with
+                                                            | inl wc' =>
+                                                              inl (conditionPair (fst wc') wc'
+                                                                                 (RtlCABool And (RtlReadWire Bool (getActionGuard name) :: RtlReadWire Bool (getActionEn name) :: nil),
+                                                                                  convertExprToRtl expr)
+                                                                  )%rtl_expr
+                                                            | inr x => 
+                                                              inl (RtlCABool And (RtlReadWire Bool (getActionGuard name) :: RtlReadWire Bool (getActionEn name) :: nil),
+                                                                   convertExprToRtl expr
+                                                                  )%rtl_expr
+                                                            end
+                                             end expr
+                                | right _ => inl (RtlReadWire Bool
+                                                              (("TYPES DONT MATCH FOR REGISTER " ++ r ++ " EXPECTED " ++ natToHexStr (size regKind) ++ " GOT " ++
+                                                                                                 natToHexStr (size k)), nil),
+                                                  RtlReadWire _ ("TYPES DONT MATCH FOR REGISTERS " ++ r ++ " EXPECTED " ++ natToHexStr (size regKind) ++ " GOT " ++
+                                                                                                   natToHexStr (size k), nil))
+                                end
+            | _ => fun _ => wc
+            end expr
+          else wc
+        end.
+    End GetRegisterWrites.
+
+    Section GetMethEns.
+      Variable meth: Attribute Signature.
+      
+      Definition argKind := fst (snd meth).
+
+      Fixpoint getMethEns k (a: ActionT (fun _ => list nat) k) (startList: list nat) : sum (RtlExpr Bool * RtlExpr argKind) (RtlExpr argKind) :=
+        match a in ActionT _ _ with
+        | Return x => inr (RtlConst (getDefaultConst _))
+        | LetExpr k' expr cont =>
+          match k' return Expr (fun _ => list nat) k' ->
+                          (fullType (fun _ => list nat) k' -> ActionT (fun _ => list nat) k) -> _ with
+          | SyntaxKind k => fun expr cont => @getMethEns _ (cont startList) (inc startList)
+          | _ => fun _ _ => inr (RtlConst (getDefaultConst _))
+          end expr cont
+        | LetAction k' a' cont =>
+          let w1 := @getMethEns _ a' (0 :: startList) in
+          let w2 := @getMethEns _ (cont startList) (inc startList) in
+          match w1, w2 with
+          | inr x, inr y => inr x
+          | inr x, inl w2' => inl w2'
+          | inl w1', inr y => inl w1'
+          | inl w1', inl w2' => inl (conditionPair (fst w2') w2' w1')%rtl_expr
+          end
+        | ReadNondet k' cont =>
+          match k' return (fullType (fun _ => list nat) k' -> ActionT (fun _ => list nat) k) -> _ with
+          | SyntaxKind k => fun cont => @getMethEns _ (cont startList) (inc startList)
+          | _ => fun _ => inr (RtlConst (getDefaultConst _))
+          end cont
+        | ReadReg r k' cont =>
+          match k' return (fullType (fun _ => list nat) k' -> ActionT (fun _ => list nat) k) -> _ with
+          | SyntaxKind k => fun cont => @getMethEns _ (cont startList) (inc startList)
+          | _ => fun _ => inr (RtlConst (getDefaultConst _))
+          end cont
+        | Assertion pred cont => @getMethEns _ cont startList
+        | Sys ls cont => @getMethEns _ cont startList
+        | IfElse pred ktf t f cont =>
+          let p := convertExprToRtl pred in
+          let wt := @getMethEns _ t (0 :: startList) in
+          let wf := @getMethEns _ f (0 :: inc startList) in
+          let wc := @getMethEns _ (cont (inc (inc startList))) (inc (inc (inc startList))) in
+          match wt, wf, wc with
+          | inr x, inr y, inr z => inr x
+          | inr x, inr y, inl wc' => inl wc'
+          | inr x, inl wf', inr z => inl (conditionPair p (invalidPair (snd wf')) wf')
+          | inl wt', inr y, inr z => inl (conditionPair p wt' (invalidPair (snd wt')))
+          | inl wt', inl wf', inr z => inl (conditionPair p wt' wf')
+          | inl wt', inr y, inl wc' => inl (conditionPair (fst wc') wc' (conditionPair p wt' (invalidPair (snd wt'))))%rtl_expr
+          | inr x, inl wf', inl wc' => inl (conditionPair (fst wc') wc' (conditionPair p (invalidPair (snd wf')) wf'))%rtl_expr
+          | inl wt', inl wf', inl wc' => inl (conditionPair (fst wc') wc'
+                                                            (conditionPair p wt' wf'))%rtl_expr
+          end
+        | WriteReg r k' expr cont =>
+          @getMethEns _ cont startList
+        | MCall f k expr cont =>
+          let wc := @getMethEns _ (cont startList) (inc startList) in
+          if string_dec f (fst meth)
+          then
+            match Kind_dec argKind (fst k) with
+            | left pf => match pf in _ = Y return Expr _ (SyntaxKind Y) -> sum (RtlExpr Bool * RtlExpr argKind) (RtlExpr argKind) with
+                         | eq_refl => fun expr =>
+                                        match wc with
+                                        | inl wc' =>
+                                          inl (conditionPair (fst wc') wc'
+                                                             (RtlCABool And (RtlReadWire Bool (getActionGuard name) :: RtlReadWire Bool (getActionEn name) :: nil),
+                                                              convertExprToRtl expr)
+                                              )%rtl_expr
+                                        | inr _ =>
+                                          inl (RtlCABool And (RtlReadWire Bool (getActionGuard name) :: RtlReadWire Bool (getActionEn name) :: nil),
+                                               convertExprToRtl expr
+                                              )%rtl_expr
+                                        end
+                         end expr
+            | right _ => inl (RtlReadWire Bool ("TYPES DONT MATCH FOR METHOD " ++ f, nil),
+                              RtlReadWire _ ("", nil))
+            end
+          else wc
+        end.
+
+    End GetMethEns.
+    Close Scope string.
+  End MethReg.
+
+  Definition convertRegsWrites regs k (a: ActionT (fun _ => list nat) k) startList :=
+    map (fun reg =>
+           let wc := getRegisterWrites reg a startList in
+           match wc with
+           | inl wc' =>
+             (getRegActionFinalWrite name (fst reg), existT _ (regKind reg)
+                                                            (RtlITE (fst wc')%rtl_expr (snd wc')%rtl_expr
+                                                                    (RtlReadWire _ (getRegActionRead name (fst reg)))))
+           | inr x => (getRegActionFinalWrite name (fst reg), existT _ (regKind reg) (RtlReadWire _ (getRegActionRead name (fst reg))))
+           end
+        ) regs.
+
+  
+  Definition getRtlDisp (d: SysT (fun _ => list nat)) :=
+    match d with
+    | DispString s => RtlDispString s
+    | DispBool e f => RtlDispBool (@convertExprToRtl _ e) f
+    | DispBit n e f => RtlDispBit (@convertExprToRtl _ e) f
+    | DispStruct n fk fs e f => RtlDispStruct (@convertExprToRtl _ e) f
+    | DispArray n k e f => RtlDispArray (@convertExprToRtl _ e) f
+    | Finish => RtlFinish
+    end.
+
+  Fixpoint getRtlSys k (a: ActionT (fun _ => list nat) k) enable startList : list (RtlExpr Bool * list RtlSysT) :=
+    match a in ActionT _ _ with
+    | MCall meth k argExpr cont =>
+      getRtlSys (cont startList) enable (inc startList)
+    | LetExpr k' expr cont =>
+      match k' return (fullType (fun _ => list nat) k' -> ActionT (fun _ => list nat) k) ->
+                      list (RtlExpr Bool * list RtlSysT) with
+      | SyntaxKind k => fun cont =>
+                          getRtlSys (cont startList) enable (inc startList)
+      | _ => fun _ => nil
+      end cont
+    | LetAction k' a' cont =>
+      getRtlSys a' enable (0 :: startList) ++
+                getRtlSys (cont startList) enable (inc startList)
+    | ReadNondet k' cont =>
+      match k' return (fullType (fun _ => list nat) k' -> ActionT (fun _ => list nat) k) ->
+                      list (RtlExpr Bool * list RtlSysT) with
+      | SyntaxKind k => fun cont =>
+                          getRtlSys (cont startList) enable (inc startList)
+      | _ => fun _ => nil
+      end cont
+    | ReadReg r k' cont =>
+      match k' return (fullType (fun _ => list nat) k' -> ActionT (fun _ => list nat) k) ->
+                      list (RtlExpr Bool * list RtlSysT) with
+      | SyntaxKind k => fun cont =>
+                          getRtlSys (cont startList) enable (inc startList)
+      | _ => fun _ => nil
+      end cont
+    | WriteReg r k' expr cont =>
+      getRtlSys cont enable startList
+    | Assertion pred cont => getRtlSys cont (RtlCABool And
+                                                       (convertExprToRtl pred :: enable :: nil))
+                                       startList
+    | Sys ls cont => (enable, map getRtlDisp ls) :: getRtlSys cont enable startList
+    | Return x => nil
+    | IfElse pred ktf t f cont =>
+      getRtlSys t (RtlCABool And (convertExprToRtl pred :: enable :: nil)) (0 :: startList) ++
+                getRtlSys f (RtlCABool And (convertExprToRtl (UniBool Neg pred) :: enable :: nil)) (0 :: inc startList) ++
+                getRtlSys (cont (inc (inc startList))) enable (inc (inc (inc startList)))
+    end.
+End Compile.
+
+Definition getRule m r :=
+  find (fun x => getBool (string_dec r (fst x))) (getRules m).
+
+Definition getMeth m r :=
+  find (fun x => getBool (string_dec r (fst x))) (getMethods m).
+
+Section ForMeth.
+  Variable m: BaseModule.
+  Variable meth: Attribute Signature.
+  Open Scope string.
+
+  Fixpoint getMethEnsOrder (order: list string) : sum (RtlExpr Bool * RtlExpr (fst (snd meth))) (RtlExpr (fst (snd meth))) :=
+    match order with
+    | o :: order' => let wc' := getMethEnsOrder order' in
+                     match getRule m o with
+                     | Some r =>
+                       let wm' := getMethEns (fst r) meth (snd r _) (1 :: nil) in
+                       match wc', wm' with
+                       | inr x, inr y => inr x
+                       | inl wc'', inr y => inl wc''
+                       | inr x, inl wm'' => inl wm''
+                       | inl wc'', inl wm'' =>
+                         inl (conditionPair (fst wc'') wc'' wm'')%rtl_expr
+                       end
+                       (* (RtlITE (wc' @% "valid") wc' *)
+                       (*         match getMethEns (fst r) meth (snd r _) (1 :: nil) with *)
+                       (*         | Some methEns => methEns *)
+                       (*         | None => invalidRtl _ *)
+                       (*         end *)
+                       (* )%rtl_expr *)
+                     | None => match getMeth m o with
+                               | Some r =>
+                                 let wm' := getMethEns (fst r) meth (projT2 (snd r) _ (1 :: nil)) (2 :: nil) in
+                                 match wc', wm' with
+                                 | inr y, inr z => inr y
+                                 | inl wc'', inr z => inl wc''
+                                 | inr y, inl wm'' => inl wm''
+                                 | inl wc'', inl wm'' =>
+                                   inl (conditionPair (fst wc'') wc'' wm'')%rtl_expr
+                                 end
+                               | None => inr (RtlConst (getDefaultConst _))
+                               end
+                     end
+    | nil => (* invalidRtl _ *) inr (RtlConst (getDefaultConst _))
+    end.
+
+  Definition getMethEnsOrderEn order :=
+    match getMethEnsOrder order with
+    | inr x => (getMethEn (fst meth), existT _ Bool (RtlConst false))%rtl_expr
+    | inl vals => (getMethEn (fst meth), existT _ Bool (fst vals))%rtl_expr
+    end.
+    (* (getMethEn (fst meth), existT _ Bool (getMethEnsRules rules @% "valid"))%rtl_expr. *)
+
+  Definition getMethEnsOrderArg order :=
+    match getMethEnsOrder order with
+    | inr x => (getMethArg (fst meth), existT _ _ x)%rtl_expr
+    | inl vals => (getMethArg (fst meth), existT _ _ (snd vals))%rtl_expr
+    end.
+    (* (getMethArg (fst meth), existT _ _ (getMethEnsRules rules @% "data"))%rtl_expr. *)
+  Close Scope string.
+End ForMeth.
+
+
+Definition getMethEnsOrderFull m order := map (fun meth => getMethEnsOrderEn m meth order) (getCallsWithSignPerMod (Base m)) ++
+                                              map (fun meth => getMethEnsOrderArg m meth order) (getCallsWithSignPerMod (Base m)).
+
+Definition getSysPerRule (rule: Attribute (Action Void)) :=
+  getRtlSys (fst rule) (snd rule (fun _ => list nat)) (RtlReadWire Bool (getActionGuard (fst rule))) (1 :: nil).
+
+Definition getSysPerMeth (meth: DefMethT) :=
+  getRtlSys (fst meth) (projT2 (snd meth) (fun _ => list nat) (1 :: nil)) (RtlReadWire Bool (getActionGuard (fst meth))) (2 :: nil).
+
+Definition getSysPerBaseMod m := concat (map getSysPerRule (getRules m) ++ map getSysPerMeth (getMethods m)).
+
+(* Set the enables correctly in the following two functions *)
+
+Definition computeRuleAssigns (r: Attribute (Action Void)) :=
+  (getActionGuard (fst r),
+   existT _ Bool (convertActionToRtl_guardF (fst r) (snd r (fun _ => list nat)) (1 :: nil)))
+    ::
+    (getActionEn (fst r), existT _ Bool (RtlReadWire Bool (getActionGuard (fst r))))
+    ::
+    convertActionToRtl_noGuard (fst r) (snd r (fun _ => list nat)) (1 :: nil) (0 :: nil).
+
+Definition computeRuleAssignsRegs regs (r: Attribute (Action Void)) :=
+  convertRegsWrites (fst r) regs (snd r (fun _ => list nat)) (1 :: nil).
+
+Definition computeMethAssigns (f: DefMethT) :=
+  (getMethGuard (fst f),
+   existT _ Bool (convertActionToRtl_guardF (fst f) (projT2 (snd f) (fun _ => list nat) (1 :: nil)) (2 :: nil)))
+    :: (fst f, (1 :: nil),
+        existT _ (fst (projT1 (snd f))) (RtlReadWire _ (getMethArg (fst f))))
+    :: (getMethRet (fst f),
+        existT _ (snd (projT1 (snd f))) (RtlReadWire _ (fst f, (0 :: nil))))
+    ::
+    convertActionToRtl_noGuard (fst f) (projT2 (snd f) (fun _ => list nat) (1 :: nil)) (2 :: nil) (0 :: nil).
+
+Definition computeMethAssignsRegs regs (f: DefMethT) :=
+  convertRegsWrites (fst f) regs (projT2 (snd f) (fun _ => list nat) (1 :: nil)) (2 :: nil).
+
+Definition getInputs (calls defs: list (Attribute (Kind * Kind))) := map (fun x => (getMethRet (fst x), snd (snd x))) calls ++
+                                                                         map (fun x => (getMethArg (fst x), fst (snd x))) defs ++
+                                                                         map (fun x => (getMethEn (fst x), Bool)) defs.
+
+Definition getInputGuards (calls: list (Attribute (Kind * Kind))) := map (fun x => (getMethGuard (fst x), Bool)) calls.
+
+Definition getOutputs (calls defs: list (Attribute (Kind * Kind))) := map (fun x => (getMethArg (fst x), fst (snd x))) calls ++
+                                                                          map (fun x => (getMethEn (fst x), Bool)) calls ++
+                                                                          map (fun x => (getMethRet (fst x), snd (snd x))) defs ++
+                                                                          map (fun x => (getMethGuard (fst x), Bool)) defs.
+
+Definition getRegInit (y: sigT RegInitValT): {x: Kind & option (ConstT x)} :=
+  existT _ _
+         match projT2 y with
+         | Uninit => None
+         | Init y' => Some match y' in ConstFullT k return ConstT match k with
+                                                                  | SyntaxKind k' => k'
+                                                                  | _ => Void
+                                                                  end with
+                           | SyntaxConst k c => c
+                           | _ => WO
+                           end
+         | RegFileUninit num k pf => None
+         | RegFileInit num k pf val =>
+           Some
+             match eq_sym pf in _ = Y return ConstT match Y with
+                                                    | SyntaxKind k' => k'
+                                                    | NativeKind _ => Void
+                                                    end with
+             | eq_refl => ConstArray (fun _ => val)
+             end
+             
+         | RegFileHex num k pf file => None
+         | RegFileBin num k pf file => None
+         end.
+
+Fixpoint getAllWriteReadConnections' (regs: list RegInitT) (order: list string) :=
+  match order with
+  | penult :: xs =>
+    match xs with
+    | ult :: ys =>
+      map (fun r => (getRegActionRead ult (fst r), existT _ _ (RtlReadWire (projT1 (getRegInit (snd r))) (getRegActionFinalWrite penult (fst r))))) regs
+          ++ getAllWriteReadConnections' regs xs
+    | nil =>
+      map (fun r => (getRegWrite (fst r), existT _ _ (RtlReadWire (projT1 (getRegInit (snd r))) (getRegActionFinalWrite penult (fst r))))) regs
+    end
+  | nil => nil
+  end.
+
+Definition getAllWriteReadConnections (regs: list RegInitT) (order: list string) :=
+  match order with
+  | beg :: xs =>
+    map (fun r => (getRegActionRead beg (fst r), existT _ _ (RtlReadWire (projT1 (getRegInit (snd r))) (getRegRead (fst r))))) regs
+        ++ getAllWriteReadConnections' regs order
+  | nil => nil
+  end.
+
+Definition getWires m (order: list string) :=
+  concat (map computeRuleAssigns (getRules m)) ++ concat (map (computeRuleAssignsRegs (getRegisters m)) (getRules m)) ++
+         concat (map computeMethAssigns (getMethods m)) ++ concat (map (computeMethAssignsRegs (getRegisters m)) (getMethods m)) ++
+         getAllWriteReadConnections (getRegisters m) order ++
+         getMethEnsOrderFull m order.
+      
+Definition getWriteRegs (regs: list RegInitT) :=
+  map (fun r => (fst r, existT _ (projT1 (getRegInit (snd r))) (RtlReadWire _ (getRegWrite (fst r))))) regs.
+
+Definition getReadRegs (regs: list RegInitT) :=
+  map (fun r => (getRegRead (fst r), existT _ (projT1 (getRegInit (snd r))) (RtlReadReg _ (fst r)))) regs.
+
+Definition filterNotInList A (f: A -> string) ls x :=
+  if In_dec string_dec (f x) ls then false else true.
+
+Definition getAllMethodsRegFileList ls :=
+  concat (map (fun x => getMethods (BaseRegFile x)) ls).
+
+Definition SubtractList A B (f: A -> string) (g: B -> string) l1 l2 :=
+  filter (filterNotInList f (map g l2)) l1.
+
+Definition setMethodGuards (ignoreMeths: list string) m :=
+  map (fun m => (getMethGuard (fst m), existT _ Bool (RtlConst (ConstBool true)))) (SubtractList fst id (getCallsWithSignPerMod (Base m)) ignoreMeths).
+
+(* Inputs and outputs must be all method calls in base module - register file methods being called *)
+(* Reg File methods definitions must serve as wires *)
+Definition getRtl_full (bm: (list string * (list RegFileBase * BaseModule))) (preserveGuards: list string) (order: list string) :=
+  {| hiddenWires := map (fun x => getMethRet x) (fst bm) ++ map (fun x => getMethArg x) (fst bm) ++ map (fun x => getMethEn x) (fst bm);
+     regFiles := map (fun x => (false, x)) (fst (snd bm));
+     inputs := getInputs (SubtractList fst fst (getCallsWithSignPerMod (Base (snd (snd bm))))
+                                       (getAllMethodsRegFileList (fst (snd bm))))
+                         (SubtractList fst fst (map (fun x => (fst x, projT1 (snd x))) (getMethods (snd (snd bm))))
+                                       (getAllMethodsRegFileList (fst (snd bm))))
+                         ++
+                         getInputGuards (filter (fun x => getBool (in_dec string_dec (fst x) preserveGuards))
+                                                (getCallsWithSignPerMod (Base (snd (snd bm)))));
+     outputs := getOutputs (SubtractList fst fst (getCallsWithSignPerMod (Base (snd (snd bm))))
+                                         (getAllMethodsRegFileList (fst (snd bm))))
+                           (SubtractList fst fst (map (fun x => (fst x, projT1 (snd x))) (getMethods (snd (snd bm))))
+                                         (getAllMethodsRegFileList (fst (snd bm))));
+     regInits := map (fun x => (fst x, getRtlRegInit (snd x))) (getRegisters (snd (snd bm)));
+     regWrites := getWriteRegs (getRegisters (snd (snd bm)));
+     wires := getReadRegs (getRegisters (snd (snd bm))) ++ getWires (snd (snd bm)) order ++
+                          setMethodGuards (map fst (getAllMethodsRegFileList (fst (snd bm))) ++ preserveGuards) (snd (snd bm));
+     sys := getSysPerBaseMod (snd (snd bm)) |}.
+
+Definition getRtl (bm: (list string * (list RegFileBase * BaseModule))) := getRtl_full bm nil (map fst (getRules (snd (snd bm)))).
+
+Definition rtlGet m pgs :=
+  getRtl_full (getHidden m, (fst (separateBaseMod m), inlineAll_All_mod (mergeSeparatedBaseMod (snd (separateBaseMod m))))) pgs (map fst (getAllRules m)).
+
+Definition makeRtl (m: ModWfOrd) pgs :=
+  getRtl_full (getHidden m, (fst (separateBaseMod m), inlineAll_All_mod (mergeSeparatedBaseMod (snd (separateBaseMod m))))) pgs (modOrd m).
