Thread.v
@@ -1,0 +1,35 @@
+Require Import List.
+
+Set Implicit Arguments.
+Set Asymmetric Patterns.
+
+Definition State (s a: Type) := s -> (a * s).
+
+Definition get {s: Type} : State s s := fun i => (i, i).
+Definition gets {s a: Type} f : State s a := fun s => (f s, s).
+Definition put {s: Type} x : State s unit := fun _ => (tt, x).
+Definition modify {s: Type} (f: s -> s): State s unit := fun i => (tt, f i).
+
+Definition bind s a b (f: State s a) (g: a -> State s b) : State s b :=
+  fun i =>
+    let (x, y) := f i in g x y.
+
+Definition ret s a (v: a) : State s a := fun i => (v, i).
+
+Definition run s a (m: State s a) init : (a * s) := m init.
+
+Notation "'do' x <- y ; cont" := (bind y (fun x => cont)) (at level 20).
+
+Section test.
+  Let MyS := State (list nat) nat.
+
+  Let ADef := 0.
+
+  Let mon := (do test <- get ;
+                do _ <- put (tail test) ;
+                do test2 <- get ;
+                ret (hd 0 test2)
+             ).
+
+  Let montest := eq_refl: (run mon (34 :: 673 :: 3 :: 84 :: nil) = (673, 673 :: 3 :: 84 :: nil)).
+End test.
